thread the model

src/Sound/Data/Ast/Expr.dfy
@@ -36,85 +36,85 @@ module Expr {
       case _ => 2
     }
 
-    function ToBinaryFunc(): (M.Any, M.Any) --> M.Any
+    function ToBinaryFunc(m: M.Model): (M.Any, M.Any) --> M.Any
       requires Arity() == 2
     {
       match this {
-        case Equiv => M.Equiv
-        case LogicalImp => M.Implies
-        case LogicalAnd => M.LogicAnd
-        case LogicalOr => M.Or
-        case Eql => M.Eql
-        case Neql => M.Neql
-        case Less => M.Less
-        case AtMost => M.AtMost
-        case Plus => M.Plus
-        case Minus => M.Minus
-        case Times => M.Times
-        case Div => M.Div
-        case Mod => M.Mod
+        case Equiv => m.Equiv
+        case LogicalImp => m.Implies
+        case LogicalAnd => m.LogicAnd
+        case LogicalOr => m.Or
+        case Eql => m.Eql
+        case Neql => m.Neql
+        case Less => m.Less
+        case AtMost => m.AtMost
+        case Plus => m.Plus
+        case Minus => m.Minus
+        case Times => m.Times
+        case Div => m.Div
+        case Mod => m.Mod
       }
     }
 
-    function ToUnaryFunc(): M.Any --> M.Any
+    function ToUnaryFunc(m: M.Model): M.Any --> M.Any
       requires Arity() == 1
     {
       match this {
-        case LogicalNot => M.Not
-        case UnaryMinus => M.Negate
+        case LogicalNot => m.Not
+        case UnaryMinus => m.Negate
       }
     }
 
-    predicate CompatibleWith(args: seq<M.Any>) {
+    predicate CompatibleWith(args: seq<M.Any>, m: M.Model) {
       |args| == Arity() &&
       match this
-      case IfThenElse => M.IsBool(args[0])
+      case IfThenElse => m.IsBool(args[0])
       case Eql | Neql => true 
       case _ => 
         if Type() == M.Int then
-          && (forall i :: 0 <= i < |args| ==> M.IsInt(args[i]))
-          && (Div? || Mod? ==> M.ToInt(args[1]) != 0)
+          && (forall i :: 0 <= i < |args| ==> m.IsInt(args[i]))
+          && (Div? || Mod? ==> m.ToInt(args[1]) != 0)
         else if Type() == M.Bool then
-          forall i :: 0 <= i < |args| ==> M.IsBool(args[i])
+          forall i :: 0 <= i < |args| ==> m.IsBool(args[i])
         else false
     }
 
-    opaque function Eval(args: seq<M.Any>): Option<M.Any>
+    opaque function Eval(args: seq<M.Any>, m: M.Model): Option<M.Any>
     {
-      if !CompatibleWith(args) then None
+      if !CompatibleWith(args, m) then None
       else if Arity() == 3 then
-        if M.IsBool(args[0]) then Some(args[0]) else Some(args[1])
+        if m.IsBool(args[0]) then Some(args[0]) else Some(args[1])
       else if Arity() == 1 then
-        Some(ToUnaryFunc()(args[0]))
+        Some(ToUnaryFunc(m)(args[0]))
       else if Arity() == 2 then
-        Some(ToBinaryFunc()(args[0], args[1]))
+        Some(ToBinaryFunc(m)(args[0], args[1]))
       else None
     }
 
-    greatest predicate RefEval(args: seq<M.Any>, outs: iset<M.Any>)
+    greatest predicate RefEval(args: seq<M.Any>, outs: iset<M.Any>, m: M.Model)
     {
-      Eval(args).Some? && Eval(args).value in outs
+      Eval(args, m).Some? && Eval(args, m).value in outs
     }
   }
 
-  lemma EqlEvalLemma(v1: M.Any, v2: M.Any)
-    ensures Eql.Eval([v1, v2]) == Some(M.InterpBool(v1 == v2))
+  lemma EqlEvalLemma(v1: M.Any, v2: M.Any, m: M.Model)
+    ensures Eql.Eval([v1, v2], m) == Some(m.InterpBool(v1 == v2))
   {
     reveal Eql.Eval;
   }
 
-  lemma AndEvalLemma(v1: M.Any, v2: M.Any)
-    requires M.IsBool(v1)
-    requires M.IsBool(v2)
-    ensures LogicalAnd.Eval([v1, v2]) == Some(M.LogicAnd(v1, v2))
+  lemma AndEvalLemma(v1: M.Any, v2: M.Any, m: M.Model)
+    requires m.IsBool(v1)
+    requires m.IsBool(v2)
+    ensures LogicalAnd.Eval([v1, v2], m) == Some(m.LogicAnd(v1, v2))
   {
     reveal LogicalAnd.Eval;
   }
 
-  lemma ImpliesEvalLemma(v1: M.Any, v2: M.Any)
-    requires M.IsBool(v1)
-    ensures LogicalImp.Eval([v1, v2]) == 
-      if M.IsBool(v2) then Some(M.Implies(v1, v2)) else None
+  lemma ImpliesEvalLemma(v1: M.Any, v2: M.Any, m: M.Model)
+    requires m.IsBool(v1)
+    ensures LogicalImp.Eval([v1, v2], m) == 
+      if m.IsBool(v2) then Some(m.Implies(v1, v2)) else None
   {
     reveal LogicalImp.Eval;
   }
@@ -161,27 +161,27 @@ module Expr {
       Definition.value.body
     }
 
-    predicate ArgsCompatibleWith(args: seq<M.Any>) {
-      |args| == |Parameters| && forall i :: 0 <= i < |args| ==> M.HasType(args[i], Parameters[i].typ.ToType())
+    predicate ArgsCompatibleWith(args: seq<M.Any>, m: M.Model) {
+      |args| == |Parameters| && forall i :: 0 <= i < |args| ==> m.HasType(args[i], Parameters[i].typ.ToType())
     }
 
     function ToFunction(): M.Function {
       M.Function(Name, seq(|Parameters|, (i: nat) requires i < |Parameters| => Parameters[i].typ.ToType()), ResultType.ToType())
     }
 
-    function EvalArgs(args: seq<M.Any>): Option<M.Any> {
-      if ArgsCompatibleWith(args) then 
-        Some(M.InterpFunctionOn(ToFunction(), args)) 
+    function EvalArgs(args: seq<M.Any>, m: M.Model): Option<M.Any> {
+      if ArgsCompatibleWith(args, m) then 
+        Some(m.InterpFunctionOn(ToFunction(), args)) 
       else None
     }
 
-    greatest predicate RefEval(args: seq<M.Any>, outs: iset<M.Any>)
+    greatest predicate RefEval(args: seq<M.Any>, outs: iset<M.Any>, m: M.Model)
       reads *
     {
-      && ArgsCompatibleWith(args)
-      && var fval := M.InterpFunctionOn(ToFunction(), args);
+      && ArgsCompatibleWith(args, m)
+      && var fval := m.InterpFunctionOn(ToFunction(), args);
         && fval in outs
-        && (!IsUninterpreted() ==> GetDef().RefEval(ToState(args), iset{fval}))
+        && (!IsUninterpreted() ==> GetDef().RefEval(ToState(args), iset{fval}, m))
     }
 
     predicate Valid()
@@ -195,13 +195,13 @@ module Expr {
     //     Eq
     // }
 
-    ghost predicate IsSound()
+    ghost predicate IsSound(m: M.Model)
       // requires Valid()
       reads *
     {
       !IsUninterpreted() ==> 
-        forall args: seq<M.Any> | ArgsCompatibleWith(args) :: 
-          GetDef().RefEval(ToState(args), iset{M.InterpFunctionOn(ToFunction(), args)})
+        forall args: seq<M.Any> | ArgsCompatibleWith(args, m) :: 
+          GetDef().RefEval(ToState(args), iset{m.InterpFunctionOn(ToFunction(), args)}, m)
     }
 
     function FunctionsCalled(): set<Function>
@@ -210,16 +210,16 @@ module Expr {
       if IsUninterpreted() then {} else GetDef().FunctionsCalled()
     }
 
-    lemma EvalSound(args: seq<M.Any>, funs: set<Function>, outs: iset<M.Any>)
-      requires EvalArgs(args).Some?
-      requires forall func <- funs :: func.IsSound()
+    lemma EvalSound(args: seq<M.Any>, funs: set<Function>, outs: iset<M.Any>, m: M.Model)
+      requires EvalArgs(args, m).Some?
+      requires forall func <- funs :: func.IsSound(m)
       requires forall func <- funs :: func.FunctionsCalled() <= funs
       requires this in funs
-      requires EvalArgs(args).value in outs
-      ensures RefEval(args, outs)
+      requires EvalArgs(args, m).value in outs
+      ensures RefEval(args, outs, m)
     {
       if !IsUninterpreted() {
-        assert ArgsCompatibleWith(args);
+        assert ArgsCompatibleWith(args, m);
         // GetDef().EvalSound(ToState(args), funs);
         // calc {
         //   RefEval(args, iset{EvalArgs(args).value});
@@ -274,225 +274,231 @@ module Expr {
       forall func <- FunctionsCalled() :: func.Valid()
     }
 
-    ghost function Eval(s: State): Option<M.Any>
+    ghost function Eval(s: State, m: M.Model): Option<M.Any>
       requires IsDefinedOn(|s|)
     {
       match this
-      case BConst(bvalue)  => Some(M.InterpBool(bvalue))
-      case IConst(ivalue)  => Some(M.InterpInt(ivalue))
+      case BConst(bvalue)  => Some(m.InterpBool(bvalue))
+      case IConst(ivalue)  => Some(m.InterpInt(ivalue))
       case BVar(id) => Some(s[id])
-      case CustomConst(value) => Some(M.InterpLiteral(value.ToLiteral()))
+      case CustomConst(value) => Some(m.InterpLiteral(value.ToLiteral()))
       case OperatorExpr(op, args) => 
-        var args :- SeqEval(args, s);
-        op.Eval(args)
+        var args :- SeqEval(args, s, m);
+        op.Eval(args, m)
       case FunctionCallExpr(func, args) => 
-        var args :- SeqEval(args, s);
-        func.EvalArgs(args)
+        var args :- SeqEval(args, s, m);
+        func.EvalArgs(args, m)
       case QuantifierExpr(true, v, typ, body) =>
-        if (forall x: M.Any | M.HasType(x, typ.ToType()) :: 
-            SomeBVal?(body.Eval(s.Update([x])))) then 
-          Some(M.InterpBool(forall x: M.Any | M.HasType(x, typ.ToType()) :: 
-            body.Eval(s.Update([x])) == Some(M.True)
+        if (forall x: M.Any | m.HasType(x, typ.ToType()) :: 
+            SomeBVal?(body.Eval(s.Update([x]), m), m)) then 
+          Some(m.InterpBool(forall x: M.Any | m.HasType(x, typ.ToType()) :: 
+            body.Eval(s.Update([x]), m) == Some(m.True())
           ))
         else None
       case QuantifierExpr(false, v, typ, body) =>
-        if (forall x: M.Any | M.HasType(x, typ.ToType()) :: 
-            SomeBVal?(body.Eval(s.Update([x])))) then 
-          Some(M.InterpBool(exists x: M.Any | M.HasType(x, typ.ToType()) :: 
-            body.Eval(s.Update([x])) == Some(M.True)
+        if (forall x: M.Any | m.HasType(x, typ.ToType()) :: 
+            SomeBVal?(body.Eval(s.Update([x]), m), m)) then 
+          Some(m.InterpBool(exists x: M.Any | m.HasType(x, typ.ToType()) :: 
+            body.Eval(s.Update([x]), m) == Some(m.True())
           ))
         else None
       case LetExpr(v, rhs, body) => 
-        var x :- rhs.Eval(s);
-        body.Eval(s.Update([x]))
+        var x :- rhs.Eval(s, m);
+        body.Eval(s.Update([x]), m)
     }
 
-    greatest predicate RefEval(s: State, outs: iset<M.Any>)
+    greatest predicate RefEval(s: State, outs: iset<M.Any>, m: M.Model)
       reads *
     {
       match this
-      case BConst(bvalue) => M.InterpBool(bvalue) in outs
-      case IConst(ivalue) => M.InterpInt(ivalue) in outs
-      case CustomConst(value) => M.InterpLiteral(value.ToLiteral()) in outs
+      case BConst(bvalue) => m.InterpBool(bvalue) in outs
+      case IConst(ivalue) => m.InterpInt(ivalue) in outs
+      case CustomConst(value) => m.InterpLiteral(value.ToLiteral()) in outs
       case BVar(id) => id < |s| && s[id] in outs
       case OperatorExpr(op, args) => 
         exists outArgsSet: seq<iset<M.Any>> :: 
-          && RefSeqEval(args, s, outArgsSet)
-          && forall outArgs <- CrossProduct(outArgsSet) :: op.RefEval(outArgs, outs)
+          && RefSeqEval(args, s, outArgsSet, m)
+          && forall outArgs <- CrossProduct(outArgsSet) :: op.RefEval(outArgs, outs, m)
       case FunctionCallExpr(func, args) => 
         exists outArgsSet: seq<iset<M.Any>> :: 
-          && RefSeqEval(args, s, outArgsSet)
-          && forall outArgs <- CrossProduct(outArgsSet) :: func.RefEval(outArgs, outs)
+          && RefSeqEval(args, s, outArgsSet, m)
+          && forall outArgs <- CrossProduct(outArgsSet) :: func.RefEval(outArgs, outs, m)
       case LetExpr(v, rhs, body) => 
         exists outsRhs: iset<M.Any> :: 
-          && rhs.RefEval(s, outsRhs)
-          && forall out <- outsRhs :: body.RefEval(s.Update([out]), outs)
+          && rhs.RefEval(s, outsRhs, m)
+          && forall out <- outsRhs :: body.RefEval(s.Update([out]), outs, m)
       case QuantifierExpr(true, v, tp, body) => 
-        (forall x: M.Any | M.HasType(x, tp.ToType()) :: 
-            body.RefEval(s.Update([x]), iset v | M.IsBool(v)))
+        (forall x: M.Any | m.HasType(x, tp.ToType()) :: 
+            body.RefEval(s.Update([x]), (iset v | m.IsBool(v)), m))
         &&
-        ((M.True in outs &&
-          forall x: M.Any | M.HasType(x, tp.ToType()) :: 
-            body.RefEval(s.Update([x]), iset{M.True}))
+        ((m.True() in outs &&
+          forall x: M.Any | m.HasType(x, tp.ToType()) :: 
+            body.RefEval(s.Update([x]), iset{m.True()}, m))
         ||
-        (M.False in outs &&
-          exists x: M.Any | M.HasType(x, tp.ToType()) :: 
-            body.RefEval(s.Update([x]), iset{M.False})))
+        (m.False() in outs &&
+          exists x: M.Any | m.HasType(x, tp.ToType()) :: 
+            body.RefEval(s.Update([x]), iset{m.False()}, m)))
       case QuantifierExpr(false, v, tp, body) =>
-        (forall x: M.Any | M.HasType(x, tp.ToType()) :: 
-            body.RefEval(s.Update([x]), iset v | M.IsBool(v)))
+        (forall x: M.Any | m.HasType(x, tp.ToType()) :: 
+            body.RefEval(s.Update([x]), (iset v | m.IsBool(v)), m))
         &&
-        ((M.True in outs &&
-          exists x: M.Any | M.HasType(x, tp.ToType()) :: 
-            body.RefEval(s.Update([x]), iset{M.True}))
+        ((m.True() in outs &&
+          exists x: M.Any | m.HasType(x, tp.ToType()) :: 
+            body.RefEval(s.Update([x]), iset{m.True()}, m))
         ||
-        (M.False in outs &&
-          forall x: M.Any | M.HasType(x, tp.ToType()) :: 
-            body.RefEval(s.Update([x]), iset{M.False})))
+        (m.False() in outs &&
+          forall x: M.Any | m.HasType(x, tp.ToType()) :: 
+            body.RefEval(s.Update([x]), iset{m.False()}, m)))
     }
 
-    ghost predicate LetRefEval(s: State, rhs: Expr, body: Expr, outsRhs: iset<M.Any>, outs: iset<M.Any>)
+    ghost predicate LetRefEval(s: State, rhs: Expr, body: Expr, outsRhs: iset<M.Any>, outs: iset<M.Any>, m: M.Model)
       reads *
     {
-      forall out <- outsRhs :: body.RefEval(s.Update([out]), outs)
+      forall out <- outsRhs :: body.RefEval(s.Update([out]), outs, m)
     }
 
-    lemma LetRefEvalUnfold(s: State, rhs: Expr, body: Expr, outs: iset<M.Any>, v: Variable) returns (outsRhs: iset<M.Any>)
-      requires LetExpr(v, rhs, body).RefEval(s, outs)
-      ensures rhs.RefEval(s, outsRhs)
-      ensures forall out <- outsRhs :: body.RefEval(s.Update([out]), outs)
+    lemma LetRefEvalUnfold(s: State, rhs: Expr, body: Expr, outs: iset<M.Any>, v: Variable, m: M.Model) returns (outsRhs: iset<M.Any>)
+      requires LetExpr(v, rhs, body).RefEval(s, outs, m)
+      ensures rhs.RefEval(s, outsRhs, m)
+      ensures forall out <- outsRhs :: body.RefEval(s.Update([out]), outs, m)
     {
-      var outsRhs' :| rhs.RefEval(s, outsRhs') &&
-        LetRefEval(s, rhs, body, outsRhs', outs);
+      var outsRhs' :| rhs.RefEval(s, outsRhs', m) &&
+        LetRefEval(s, rhs, body, outsRhs', outs, m);
       outsRhs := outsRhs';
-      forall out | out in outsRhs ensures body.RefEval(s.Update([out]), outs) {
-        assert LetRefEval(s, rhs, body, outsRhs, outs) ==> forall out <- outsRhs :: body.RefEval(s.Update([out]), outs);
+      forall out | out in outsRhs ensures body.RefEval(s.Update([out]), outs, m) {
+        assert LetRefEval(s, rhs, body, outsRhs, outs, m) ==> forall out <- outsRhs :: body.RefEval(s.Update([out]), outs, m);
       }
     }
 
-    lemma EvalComplete(s: State, outs: iset<M.Any>)
-      requires RefEval(s, outs)
+    lemma EvalComplete(s: State, outs: iset<M.Any>, m: M.Model)
+      requires RefEval(s, outs, m)
       // ensures outs != iset{}
       ensures IsDefinedOn(|s|)
-      ensures Eval(s).Some? 
-      ensures Eval(s).value in outs
+      ensures Eval(s, m).Some? 
+      ensures Eval(s, m).value in outs
     {
       match this
       case OperatorExpr(op, args) => 
         var outArgsSet :| 
-          && RefSeqEval(args, s, outArgsSet)
-          && (forall outArgs <- CrossProduct(outArgsSet) :: op.RefEval(outArgs, outs));
-        SeqEvalComplete(args, s, outArgsSet);
+          && RefSeqEval(args, s, outArgsSet, m)
+          && (forall outArgs <- CrossProduct(outArgsSet) :: op.RefEval(outArgs, outs, m));
+        SeqEvalComplete(args, s, outArgsSet, m);
       case FunctionCallExpr(func, args) => 
         var outArgsSet :| 
-          && RefSeqEval(args, s, outArgsSet)
-          && (forall outArgs <- CrossProduct(outArgsSet) :: func.RefEval(outArgs, outs));
-        SeqEvalComplete(args, s, outArgsSet);
+          && RefSeqEval(args, s, outArgsSet, m)
+          && (forall outArgs <- CrossProduct(outArgsSet) :: func.RefEval(outArgs, outs, m));
+        SeqEvalComplete(args, s, outArgsSet, m);
       case LetExpr(v, rhs, body) => 
-        var outsRhs := LetRefEvalUnfold(s, rhs, body, outs, v);
-        rhs.EvalComplete(s, outsRhs);
+        var outsRhs := LetRefEvalUnfold(s, rhs, body, outs, v, m);
+        rhs.EvalComplete(s, outsRhs, m);
       case QuantifierExpr(true, v, tp, body) => 
-        var x := M.NoEmptyTypes(tp.ToType());
+        var x := m.NoEmptyTypes(tp.ToType());
+        if (forall x: M.Any | m.HasType(x, tp.ToType()) :: 
+          body.RefEval(s.Update([x]), iset{m.True()}, m)) {
+        }
       case QuantifierExpr(false, v, tp, body) => 
-        var x := M.NoEmptyTypes(tp.ToType());
+        var x := m.NoEmptyTypes(tp.ToType());
+        if (exists x: M.Any | m.HasType(x, tp.ToType()) :: 
+          body.RefEval(s.Update([x]), iset{m.True()}, m)) {
+        }
       case _ => 
     }
 
-    lemma EvalSound(s: State, funs: set<Function>, outs: iset<M.Any>)
+    lemma EvalSound(s: State, funs: set<Function>, outs: iset<M.Any>, m: M.Model)
       requires FunctionsCalled() <= funs
-      requires forall func <- funs :: func.IsSound()
+      requires forall func <- funs :: func.IsSound(m)
       requires forall func <- funs :: func.FunctionsCalled() <= funs
       requires IsDefinedOn(|s|)
-      requires Eval(s).Some?
-      requires Eval(s).value in outs
-      ensures RefEval(s, outs)
+      requires Eval(s, m).Some?
+      requires Eval(s, m).value in outs
+      ensures RefEval(s, outs, m)
     {
       match this
       case OperatorExpr(op, args) => 
-        SeqEvalSound(args, s, funs, SeqSingleton(SeqEval(args, s).value));
-        CrossProductSeqSingleton(SeqEval(args, s).value);
+        SeqEvalSound(args, s, funs, SeqSingleton(SeqEval(args, s, m).value), m);
+        CrossProductSeqSingleton(SeqEval(args, s, m).value);
       case FunctionCallExpr(func, args) => 
-        SeqEvalSound(args, s, funs, SeqSingleton(SeqEval(args, s).value));
-        CrossProductSeqSingleton(SeqEval(args, s).value);
-        func.EvalSound(SeqEval(args, s).value, funs, outs);
-      case LetExpr(v, rhs, body) => rhs.EvalSound(s, funs, iset{rhs.Eval(s).value});
+        SeqEvalSound(args, s, funs, SeqSingleton(SeqEval(args, s, m).value), m);
+        CrossProductSeqSingleton(SeqEval(args, s, m).value);
+        func.EvalSound(SeqEval(args, s, m).value, funs, outs, m );
+      case LetExpr(v, rhs, body) => rhs.EvalSound(s, funs, iset{rhs.Eval(s, m).value}, m);
       case QuantifierExpr(true, v, typ, body) => 
-        assert forall x: M.Any | M.HasType(x, typ.ToType()) :: 
-          SomeBVal?(body.Eval(s.Update(Singleton(x))));
-        if !(forall x: M.Any | M.HasType(x, typ.ToType()) :: 
-          body.Eval(s.Update(Singleton(x))) == Some(M.True)) {
-          var x: M.Any :| M.HasType(x, typ.ToType()) &&
-            body.Eval(s.Update(Singleton(x))) != Some(M.True);
-          M.BoolIsTrueOrFalse(body.Eval(s.Update(Singleton(x))).value);
+        assert forall x: M.Any | m.HasType(x, typ.ToType()) :: 
+          SomeBVal?(body.Eval(s.Update(Singleton(x)), m), m);
+        if !(forall x: M.Any | m.HasType(x, typ.ToType()) :: 
+          body.Eval(s.Update(Singleton(x)), m) == Some(m.True())) {
+          var x: M.Any :| m.HasType(x, typ.ToType()) &&
+            body.Eval(s.Update(Singleton(x)), m) != Some(m.True());
+          m.BoolIsTrueOrFalse(body.Eval(s.Update(Singleton(x)), m).value);
         }
       case QuantifierExpr(false, v, tp, body) => 
-        assert forall x: M.Any | M.HasType(x, tp.ToType()) :: 
-          SomeBVal?(body.Eval(s.Update(Singleton(x))));
-        if !(exists x: M.Any | M.HasType(x, tp.ToType()) :: 
-          body.Eval(s.Update(Singleton(x))) == Some(M.True)) {
-          forall x: M.Any | M.HasType(x, tp.ToType()) {
-            M.BoolIsTrueOrFalse(body.Eval(s.Update(Singleton(x))).value);
+        assert forall x: M.Any | m.HasType(x, tp.ToType()) :: 
+          SomeBVal?(body.Eval(s.Update(Singleton(x)), m), m);
+        if !(exists x: M.Any | m.HasType(x, tp.ToType()) :: 
+          body.Eval(s.Update(Singleton(x)), m) == Some(m.True())) {
+          forall x: M.Any | m.HasType(x, tp.ToType()) {
+            m.BoolIsTrueOrFalse(body.Eval(s.Update(Singleton(x)), m).value);
           }
         }
       case _ =>
     }
 
-    ghost predicate HoldsOn(s: State) 
+    ghost predicate HoldsOn(s: State, m: M.Model) 
       requires IsDefinedOn(|s|)
     {
-      Eval(s) == Some(M.True)
+      Eval(s, m) == Some(m.True())
     }
 
-    ghost predicate RefHoldsOn(s: State)
+    ghost predicate RefHoldsOn(s: State, m: M.Model)
       reads *
     {
-      RefEval(s, iset{M.True})
+      RefEval(s, iset{m.True()}, m)
     }
 
-    lemma HoldsOnSound(s: State, funs: set<Function>)
+    lemma HoldsOnSound(s: State, funs: set<Function>, m: M.Model)
       requires FunctionsCalled() <= funs
-      requires forall func <- funs :: func.IsSound()
+      requires forall func <- funs :: func.IsSound(m)
       requires forall func <- funs :: func.FunctionsCalled() <= funs
-      ensures (IsDefinedOn(|s|) && HoldsOn(s)) == RefHoldsOn(s)
+      ensures (IsDefinedOn(|s|) && HoldsOn(s, m)) == RefHoldsOn(s, m)
     {
-      if IsDefinedOn(|s|) && HoldsOn(s) {
-        EvalSound(s, funs, iset{M.True});
+      if IsDefinedOn(|s|) && HoldsOn(s, m) {
+        EvalSound(s, funs, iset{m.True()}, m);
       }
-      if RefHoldsOn(s) {
-        EvalComplete(s, iset{M.True});
+      if RefHoldsOn(s, m) {
+        EvalComplete(s, iset{m.True()}, m);
       }
     }
 
-    lemma EvalDepthLemma(s1: State, s2: State) 
+    lemma EvalDepthLemma(s1: State, s2: State, m: M.Model) 
       requires IsDefinedOn(|s1|)
       requires IsDefinedOn(|s2|)
       requires forall i: Idx :: i < Depth() ==> s1[i] == s2[i]
-      ensures Eval(s1) == Eval(s2)
+      ensures Eval(s1, m) == Eval(s2, m)
     { 
       match this
       case QuantifierExpr(true, v, tp, body) => 
       case QuantifierExpr(false, v, tp, body) => 
-      case FunctionCallExpr(func, args) => SeqEvalDepthLemma(args, s1, s2);
-      case OperatorExpr(op, args) => SeqEvalDepthLemma(args, s1, s2);
+      case FunctionCallExpr(func, args) => SeqEvalDepthLemma(args, s1, s2, m);
+      case OperatorExpr(op, args) => SeqEvalDepthLemma(args, s1, s2, m);
       case _ =>
     } 
 
-    ghost predicate Holds() 
+    ghost predicate Holds(md: M.Model) 
       // reads *
     {
-      forall s: State :: IsDefinedOn(|s|) ==> HoldsOn(s)
+      forall s: State :: IsDefinedOn(|s|) ==> HoldsOn(s, md)
     }
 
-    ghost predicate RefHolds()
+    ghost predicate RefHolds(md: M.Model)
       reads *
     {
-      forall s: State :: IsDefinedOn(|s|) ==> RefHoldsOn(s)
+      forall s: State :: IsDefinedOn(|s|) ==> RefHoldsOn(s, md)
     }
 
-    ghost function Sem(): iset<State> 
+    ghost function Sem(m: M.Model): iset<State> 
       // reads *
     { 
-      iset st: State | IsDefinedOn(|st|) && HoldsOn(st) 
+      iset st: State | IsDefinedOn(|st|) && HoldsOn(st, m) 
     }
   }
 
@@ -527,45 +533,45 @@ module Expr {
     forall s <- CrossProduct(SeqSingleton(ss)) ensures s == ss { }
   }
 
-  greatest predicate RefSeqEval(ss: seq<Expr>, s: State, outSeqs: seq<iset<M.Any>>) 
+  greatest predicate RefSeqEval(ss: seq<Expr>, s: State, outSeqs: seq<iset<M.Any>>, m: M.Model) 
     reads *
   {
     if ss == [] then outSeqs == [] else
     && |outSeqs| > 0
-    && ss[0].RefEval(s, outSeqs[0])
-    && RefSeqEval(ss[1..], s, outSeqs[1..])
+    && ss[0].RefEval(s, outSeqs[0], m)
+    && RefSeqEval(ss[1..], s, outSeqs[1..], m)
   }
 
-  ghost function SeqEval(ss: seq<Expr>, s: State): Option<seq<M.Any>>
+  ghost function SeqEval(ss: seq<Expr>, s: State, m: M.Model): Option<seq<M.Any>>
     requires forall e <- ss :: e.IsDefinedOn(|s|)
-    ensures SeqEval(ss, s).Some? ==> |SeqEval(ss, s).value| == |ss|
+    ensures SeqEval(ss, s, m).Some? ==> |SeqEval(ss, s, m).value| == |ss|
   {
     if ss == [] then Some([]) else
-    var e :- ss[0].Eval(s);
-    var es :- SeqEval(ss[1..], s);
+    var e :- ss[0].Eval(s, m);
+    var es :- SeqEval(ss[1..], s, m);
     Some([e] + es)
   }
 
-  predicate ISetOptionEq<T(!new)>(x: Option<T>, y: iset<T>)
+  predicate ISetOptionEq<T(!new)>(x: Option<T>, y: iset<T>, m: M.Model)
   {
     if x.None? then false else x.value in y
   }
 
-  ghost predicate SeqISetOptionEq<T(!new)>(x: Option<seq<T>>, y: seq<iset<T>>)
+  ghost predicate SeqISetOptionEq<T(!new)>(x: Option<seq<T>>, y: seq<iset<T>>, m: M.Model)
   {
     if x.None? then false else
     x.value in CrossProduct(y) 
   }
 
-  lemma SeqEvalComplete(ss: seq<Expr>, s: State, outs: seq<iset<M.Any>>)
-    requires RefSeqEval(ss, s, outs)
+  lemma SeqEvalComplete(ss: seq<Expr>, s: State, outs: seq<iset<M.Any>>, m: M.Model)
+    requires RefSeqEval(ss, s, outs, m)
     ensures SeqExprDepth(ss) <= |s|
-    ensures SeqEval(ss, s).Some?
-    ensures SeqEval(ss, s).value in CrossProduct(outs)
+    ensures SeqEval(ss, s, m).Some?
+    ensures SeqEval(ss, s, m).value in CrossProduct(outs)
   {
     if ss != [] {
-      ss[0].EvalComplete(s, outs[0]);
-      SeqEvalComplete(ss[1..], s, outs[1..]);
+      ss[0].EvalComplete(s, outs[0], m);
+      SeqEvalComplete(ss[1..], s, outs[1..], m);
       var o :| o in outs[0];
       var os :| os in CrossProduct(outs[1..]);
       assert [o] + os in CrossProduct(outs);
@@ -574,68 +580,68 @@ module Expr {
     }
   }
 
-  lemma SeqEvalSound(ss: seq<Expr>, s: State, funs: set<Function>, outs: seq<iset<M.Any>>)
+  lemma SeqEvalSound(ss: seq<Expr>, s: State, funs: set<Function>, outs: seq<iset<M.Any>>, m: M.Model)
     requires forall e <- ss :: e.IsDefinedOn(|s|)
-    requires forall func <- funs :: func.IsSound()
+    requires forall func <- funs :: func.IsSound(m)
     requires forall func <- funs :: func.FunctionsCalled() <= funs
-    requires SeqEval(ss, s).Some?
+    requires SeqEval(ss, s, m).Some?
     requires SeqExprFunctionsCalled(ss) <= funs
-    requires SeqEval(ss, s).value in CrossProduct(outs)
-    ensures RefSeqEval(ss, s, outs)
+    requires SeqEval(ss, s, m).value in CrossProduct(outs)
+    ensures RefSeqEval(ss, s, outs, m)
   {
     if ss != [] {
-      ss[0].EvalSound(s, funs, outs[0]);
-      SeqEvalSound(ss[1..], s, funs, outs[1..]);
-      SeqSingletonCons(ss[0].Eval(s).value, SeqEval(ss[1..], s).value);
+      ss[0].EvalSound(s, funs, outs[0], m);
+      SeqEvalSound(ss[1..], s, funs, outs[1..], m);
+      SeqSingletonCons(ss[0].Eval(s, m).value, SeqEval(ss[1..], s, m).value);
     }
   }
 
-  lemma SeqEval1(e: Expr, s: State)
+  lemma SeqEval1(e: Expr, s: State, m: M.Model)
     requires e.IsDefinedOn(|s|)
-    requires e.Eval(s).Some?
-    ensures SeqEval([e], s) == Some([e.Eval(s).value])
+    requires e.Eval(s, m).Some?
+    ensures SeqEval([e], s, m) == Some([e.Eval(s, m).value])
   {
     calc {
-      SeqEval([e], s);
+      SeqEval([e], s, m);
       == { assert [e][1..] == [];
            assert [e][0] == e; }
-      Some([e.Eval(s).value] + []);
-      == { assert [e.Eval(s).value] + [] == [e.Eval(s).value]; }
-      Some([e.Eval(s).value]);
+      Some([e.Eval(s, m).value] + []);
+      == { assert [e.Eval(s, m).value] + [] == [e.Eval(s, m).value]; }
+      Some([e.Eval(s, m).value]);
     }
   }
 
-  lemma SeqEval2(e1: Expr, e2: Expr, s: State)
+  lemma SeqEval2(e1: Expr, e2: Expr, s: State, m: M.Model)
     requires e1.IsDefinedOn(|s|)
     requires e2.IsDefinedOn(|s|)
-    requires e1.Eval(s).Some?
-    requires e2.Eval(s).Some?
-    ensures SeqEval([e1, e2], s) == Some([e1.Eval(s).value, e2.Eval(s).value])
+    requires e1.Eval(s, m).Some?
+    requires e2.Eval(s, m).Some?
+    ensures SeqEval([e1, e2], s, m) == Some([e1.Eval(s, m).value, e2.Eval(s, m).value])
   {
     assert [e1, e2][1..] == [e2];
     assert [e1, e2][0] == e1;
-    SeqEval1(e2, s); 
+    SeqEval1(e2, s, m); 
     calc {
-      SeqEval([e1, e2], s);
+      SeqEval([e1, e2], s, m);
       == { assert [e1, e2][1..] == [e2];
            assert [e1, e2][0] == e1;
-           SeqEval1(e2, s); }
-      Some([e1.Eval(s).value] + SeqEval([e2], s).value);
-      == { SeqEval1(e2, s);
-           assert [e1.Eval(s).value] + [e2.Eval(s).value] == [e1.Eval(s).value, e2.Eval(s).value]; }
-      Some([e1.Eval(s).value, e2.Eval(s).value]);
+           SeqEval1(e2, s, m); }
+      Some([e1.Eval(s, m).value] + SeqEval([e2], s, m).value);
+      == { SeqEval1(e2, s, m);
+           assert [e1.Eval(s, m).value] + [e2.Eval(s, m).value] == [e1.Eval(s, m).value, e2.Eval(s, m).value]; }
+      Some([e1.Eval(s, m).value, e2.Eval(s, m).value]);
     }
   }
 
-  lemma SeqEvalDepthLemma(ss: seq<Expr>, s1: State, s2: State)
+  lemma SeqEvalDepthLemma(ss: seq<Expr>, s1: State, s2: State, m: M.Model)
     requires SeqExprDepth(ss) <= |s1|
     requires SeqExprDepth(ss) <= |s2|
     requires forall i: Idx :: i < SeqExprDepth(ss) ==> s1[i] == s2[i]
-    ensures SeqEval(ss, s1) == SeqEval(ss, s2)
+    ensures SeqEval(ss, s1, m) == SeqEval(ss, s2, m)
   {
     if ss != [] {
-      ss[0].EvalDepthLemma(s1, s2);
-      SeqEvalDepthLemma(ss[1..], s1, s2);
+      ss[0].EvalDepthLemma(s1, s2, m);
+      SeqEvalDepthLemma(ss[1..], s1, s2, m);
     }
   }
 
@@ -669,26 +675,26 @@ module Expr {
     }
   }
 
-  lemma EvalEqLemma(e1: Expr, e2: Expr, s: State)
+  lemma EvalEqLemma(e1: Expr, e2: Expr, s: State, m: M.Model)
     requires e1.IsDefinedOn(|s|)
     requires e2.IsDefinedOn(|s|)
-    requires e1.Eval(s) == e2.Eval(s)
-    requires e1.Eval(s).Some?
+    requires e1.Eval(s, m) == e2.Eval(s, m)
+    requires e1.Eval(s, m).Some?
     ensures Eq(e1, e2).Depth() == max(e1.Depth(), e2.Depth())
     ensures Eq(e1, e2).IsDefinedOn(|s|)
-    ensures Eq(e1, e2).HoldsOn(s)
+    ensures Eq(e1, e2).HoldsOn(s, m)
   { 
     SeqMaxPairLemma(e1, e2);
     calc {
-      Eq(e1, e2).Eval(s);
+      Eq(e1, e2).Eval(s, m);
       ==
-      OperatorExpr(Eql, [e1, e2]).Eval(s);
-      == { SeqEval2(e1, e2, s); }
-      Eql.Eval([e1.Eval(s).value, e2.Eval(s).value]);
-      == { EqlEvalLemma(e1.Eval(s).value, e2.Eval(s).value); }
-      Some(M.InterpBool(e1.Eval(s).value == e2.Eval(s).value));
-      == { assert e1.Eval(s) == e2.Eval(s); }
-      Some(M.InterpBool(true));
+      OperatorExpr(Eql, [e1, e2]).Eval(s, m);
+      == { SeqEval2(e1, e2, s, m); }
+      Eql.Eval([e1.Eval(s, m).value, e2.Eval(s, m).value], m);
+      == { EqlEvalLemma(e1.Eval(s, m).value, e2.Eval(s, m).value, m); }
+      Some(m.InterpBool(e1.Eval(s, m).value == e2.Eval(s, m).value));
+      == { assert e1.Eval(s, m) == e2.Eval(s, m); }
+      Some(m.InterpBool(true));
     }
   }
 
@@ -716,42 +722,42 @@ module Expr {
     SeqMaxPairLemma(e0, e1);
   }
 
-  lemma HoldsOnAndLemma(e0: Expr, e1: Expr, s: State)
+  lemma HoldsOnAndLemma(e0: Expr, e1: Expr, s: State, m: M.Model)
     requires e0.IsDefinedOn(|s|)
     requires e1.IsDefinedOn(|s|)
-    requires e0.HoldsOn(s)
-    requires e1.HoldsOn(s)
+    requires e0.HoldsOn(s, m)
+    requires e1.HoldsOn(s, m)
     ensures And(e0, e1).IsDefinedOn(|s|) 
-    ensures And(e0, e1).HoldsOn(s)
+    ensures And(e0, e1).HoldsOn(s, m)
   {
     SeqMaxPairLemma(e0, e1);
-    SeqEval2(e0, e1, s);
-    AndEvalLemma(e0.Eval(s).value, e1.Eval(s).value);
+    SeqEval2(e0, e1, s, m);
+    AndEvalLemma(e0.Eval(s, m).value, e1.Eval(s, m).value, m);
   }
 
-  lemma HoldsOnImpliesLemma(e0: Expr, e1: Expr, s: State)
+  lemma HoldsOnImpliesLemma(e0: Expr, e1: Expr, s: State, m: M.Model)
     requires e0.IsDefinedOn(|s|)
     requires e1.IsDefinedOn(|s|)
-    requires e0.HoldsOn(s)
+    requires e0.HoldsOn(s, m)
     requires (
       IsDefinedOnImpliesLemma(e0, e1, s);
-      Implies(e0, e1).HoldsOn(s))
-    ensures e1.HoldsOn(s)
+      Implies(e0, e1).HoldsOn(s, m))
+    ensures e1.HoldsOn(s, m)
   {
     IsDefinedOnImpliesLemma(e0, e1, s);
-    assert e0.Eval(s).Some?;
-    assert SeqEval([e0, e1], s).Some?;
-    if e1.Eval(s).Some? {
-      SeqEval2(e0, e1, s);
+    assert e0.Eval(s, m).Some?;
+    assert SeqEval([e0, e1], s, m).Some?;
+    if e1.Eval(s, m).Some? {
+      SeqEval2(e0, e1, s, m);
       calc {
-        Implies(e0, e1).Eval(s).value;
-        == { SeqEval2(e0, e1, s);
-             ImpliesEvalLemma(e0.Eval(s).value, e1.Eval(s).value); }
-        M.Implies(e0.Eval(s).value, e1.Eval(s).value);
+        Implies(e0, e1).Eval(s, m).value;
+        == { SeqEval2(e0, e1, s, m);
+             ImpliesEvalLemma(e0.Eval(s, m).value, e1.Eval(s, m).value, m); }
+        m.Implies(e0.Eval(s, m).value, e1.Eval(s, m).value);
         ==
-        M.Implies(M.True, e1.Eval(s).value);
+        m.Implies(m.True(), e1.Eval(s, m).value);
         ==
-         M.InterpBool(true ==> M.ToBool(e1.Eval(s).value));
+         m.InterpBool(true ==> m.ToBool(e1.Eval(s, m).value));
       }
     }
   }
@@ -788,15 +794,15 @@ module Expr {
     }
   }
 
-  lemma EvalConjLemma(ctx: seq<Expr>, s: State)
+  lemma EvalConjLemma(ctx: seq<Expr>, s: State, m: M.Model)
     requires forall e <- ctx :: e.IsDefinedOn(|s|)
-    requires forall e <- ctx :: e.HoldsOn(s)
+    requires forall e <- ctx :: e.HoldsOn(s, m)
     ensures Conj(ctx).IsDefinedOn(|s|)
-    ensures Conj(ctx).HoldsOn(s)
+    ensures Conj(ctx).HoldsOn(s, m)
   {  
     if ctx != [] { 
       IsDefinedOnAndLemma(ctx[0], Conj(ctx[1..]), s); 
-      HoldsOnAndLemma(ctx[0], Conj(ctx[1..]), s);
+      HoldsOnAndLemma(ctx[0], Conj(ctx[1..]), s, m);
     }  
   }
 
