src/Sound/Data/State/Model.dfy
@@ -2,13 +2,15 @@ module Model {
   import opened Utils
   export
     provides Utils,
-      InterpLiteral, InferType, Bot,
-      InterpInt, InterpBool, ToInt, ToBool,
-      Not, Equiv, Or, Negate, Plus, Minus, Times, Div, Mod, Less, 
-      AtMost, NoEmptyTypes, InterpFunctionOn, BoolIsTrueOrFalse, TrueNotFalse
-    reveals Any, True, False, LogicAnd, IsBool, IsInt, HasType, Implies, 
-      Literal, FunctionSig, Function, Type, Int, Bool, Eql, Neql, IsBoolSet, IsIntSet,
-      HaveTypes
+      PreModel, PreModel.InferType, PreModel.Valid,
+      PreModel.InterpLiteral,
+      PreModel.InterpInt, PreModel.InterpBool, PreModel.ToInt, PreModel.ToBool,
+      PreModel.Not, PreModel.Equiv, PreModel.Or, PreModel.Negate, PreModel.Plus, PreModel.Minus, PreModel.Times, PreModel.Div, PreModel.Mod, PreModel.Less, 
+      PreModel.AtMost, PreModel.NoEmptyTypes, PreModel.InterpFunctionOn, PreModel.BoolIsTrueOrFalse, PreModel.TrueNotFalse
+    reveals Any, Model,  Bot, PreModel,
+      PreModel.True, PreModel.False, PreModel.LogicAnd, PreModel.IsBool, PreModel.IsInt, PreModel.HasType, PreModel.Implies, 
+      Literal, FunctionSig, Function, Type, Int, Bool, PreModel.Eql, PreModel.Neql,
+      PreModel.HaveTypes
 
   type Type = string
   const Int : Type := "int"
@@ -21,166 +23,256 @@ module Model {
 
   function {:axiom} Bot(): Any
 
-  function {:axiom} InferType(x: Any): Type
+
+  datatype PreModel = Model(
+    inferType: Any -> Type,
+    interpLiteral: Literal -> Any,
+    interpInt: int -> Any,
+    interpBool: bool -> Any,
+    toInt: Any --> int,
+    toBool: Any --> bool,
+    interpFunctionOn: (Function, seq<Any>) --> Any
+    ) {
+
+    ghost opaque predicate Valid() {
+      && (forall typ: Type :: exists x: Any :: HasType(x, typ))
+      && (forall x: Literal :: HasType(interpLiteral(x), x.typ))
+      && (forall x: int :: HasType(interpInt(x), Int))
+      && (forall x: bool :: HasType(interpBool(x), Bool))
+      && (forall x: Any :: IsInt(x) ==> toInt.requires(x))
+      && (forall x: Any :: IsBool(x) ==> toBool.requires(x))
+      && (forall x: Any :: IsInt(x) ==> interpInt(toInt(x)) == x)
+      && (forall x: Any :: IsBool(x) ==> interpBool(toBool(x)) == x)
+      && (interpBool(true) != interpBool(false))
+      && (forall func: Function, args: seq<Any> :: HaveTypes(args, func.sig) ==> interpFunctionOn.requires(func, args))
+      && (forall func: Function, args: seq<Any> :: HaveTypes(args, func.sig) ==> HasType(interpFunctionOn(func, args), func.resultType))
+    }
+    function InferType(x: Any): Type
+    {
+      inferType(x)
+    }
+    
+    predicate HasType(x: Any, typ: Type) {
+      InferType(x) == typ
+    }
+
+    lemma NoEmptyTypes(typ: Type) returns (x: Any)
+      requires Valid()
+      ensures HasType(x, typ)
+    {
+      assert (forall typ: Type :: exists x: Any :: HasType(x, typ)) by {
+        reveal Valid;
+      }
+      var x': Any :| HasType(x', typ);
+      x := x';
+    }
+
+    opaque function InterpLiteral(x: Literal): Any
+      requires Valid()
+      ensures HasType(InterpLiteral(x), x.typ)
+    {
+      reveal Valid;
+      interpLiteral(x)
+    }
+
+    predicate IsInt(x: Any) {
+      HasType(x, Int)
+    }
+
+    predicate IsBool(x: Any) {
+      HasType(x, Bool)
+    }
+
+    opaque function InterpInt(x: int): Any
+      requires Valid()
+      ensures HasType(InterpInt(x), Int)
+    {
+      reveal Valid;
+      interpInt(x)
+    }
+
+    opaque function InterpBool(x: bool): Any
+      requires Valid()
+      ensures HasType(InterpBool(x), Bool)
+    {
+      reveal Valid;
+      interpBool(x)
+    }
+
+    opaque function ToBool(x: Any): bool
+      requires Valid()
+      requires IsBool(x)
+      ensures InterpBool(ToBool(x)) == x
+    {
+      reveal Valid;
+      reveal InterpBool;
+      toBool(x)
+    }
+
+    opaque function ToInt(x: Any): int
+      requires Valid()
+      requires IsInt(x)
+      ensures InterpInt(ToInt(x)) == x
+    {
+      reveal Valid;
+      reveal InterpInt;
+      toInt(x)
+    }
+
+    function True(): Any requires Valid() { InterpBool(true) }
+    function False(): Any requires Valid() { InterpBool(false) }
+
+    lemma TrueNotFalse()
+      requires Valid()
+      ensures True() != False()
+    {
+      reveal Valid;
+      reveal InterpBool;
+    }
+
+    function Eql(x: Any, y: Any): Any 
+      requires Valid()
+    {
+      InterpBool(x == y)
+    }
+
+    function Neql(x: Any, y: Any): Any 
+      requires Valid()
+    {
+      InterpBool(x != y)
+    }
+
+    function Not(x: Any): Any
+      requires Valid()
+      requires IsBool(x)
+    {
+      InterpBool(!ToBool(x))
+    }
+
+    function LogicAnd(x: Any, y: Any): Any
+      requires Valid()
+      requires IsBool(x)
+      requires IsBool(y)
+    {
+      InterpBool(ToBool(x) && ToBool(y))
+    }
+
+    function Implies(x: Any, y: Any): Any
+      requires Valid()
+      requires IsBool(x)
+      requires IsBool(y)
+    {
+      InterpBool(ToBool(x) ==> ToBool(y))
+    }
+
+    function Equiv(x: Any, y: Any): Any
+      requires Valid()
+      requires IsBool(x)
+      requires IsBool(y)
+    {
+      InterpBool(ToBool(x) <==> ToBool(y))
+    }
+
+    function Or(x: Any, y: Any): Any
+      requires Valid()
+      requires IsBool(x)
+      requires IsBool(y)
+    {
+      InterpBool(ToBool(x) || ToBool(y))
+    }
+
+    function Negate(x: Any): Any
+      requires Valid()
+      requires IsInt(x)
+    {
+      InterpInt(-ToInt(x))
+    }
+
+    function Plus(x: Any, y: Any): Any
+      requires Valid()
+      requires IsInt(x)
+      requires IsInt(y)
+    {
+      InterpInt(ToInt(x) + ToInt(y))
+    }
+
+    function Minus(x: Any, y: Any): Any
+      requires Valid()
+      requires IsInt(x)
+      requires IsInt(y)
+    {
+      InterpInt(ToInt(x) - ToInt(y))
+    }
+
+    function Times(x: Any, y: Any): Any
+      requires Valid()
+      requires IsInt(x)
+      requires IsInt(y)
+    {
+      InterpInt(ToInt(x) * ToInt(y))
+    }
+
+    function Div(x: Any, y: Any): Any
+      requires Valid()
+      requires IsInt(x)
+      requires IsInt(y)
+      requires ToInt(y) != 0
+    {
+      InterpInt(ToInt(x) / ToInt(y))
+    }
+
+    function Mod(x: Any, y: Any): Any
+      requires Valid()
+      requires IsInt(x)
+      requires IsInt(y)
+      requires ToInt(y) != 0
+    {
+      InterpInt(ToInt(x) % ToInt(y))
+    }
+
+    function Less(x: Any, y: Any): Any
+      requires Valid()
+      requires IsInt(x)
+      requires IsInt(y)
+    {
+      InterpBool(ToInt(x) < ToInt(y))
+    }
+
+    function AtMost(x: Any, y: Any): Any
+      requires Valid()
+      requires IsInt(x)
+      requires IsInt(y)
+    {
+      InterpBool(ToInt(x) <= ToInt(y))
+    }
+
+    predicate HaveTypes(args: seq<Any>, sig: FunctionSig) {
+      |args| == |sig| && forall i :: 0 <= i < |args| ==> HasType(args[i], sig[i])
+    }
+
+    opaque function InterpFunctionOn(func: Function, args: seq<Any>): Any
+      requires Valid()
+      requires HaveTypes(args, func.sig)
+      ensures HasType(InterpFunctionOn(func, args), func.resultType)
+    {
+      reveal Valid;
+      interpFunctionOn(func, args)
+    }
+
+    lemma BoolIsTrueOrFalse(x: Any)
+      requires Valid()
+      requires IsBool(x)
+      ensures x == True() || x == False()
+    {
+      reveal Valid;
+      reveal InterpBool;
+      assert x == InterpBool(ToBool(x));
+    }
+  }
+    
   
-  predicate HasType(x: Any, typ: Type) {
-    InferType(x) == typ
-  }
+  type Model = m: PreModel | m.Valid() witness *
 
-  lemma {:axiom} NoEmptyTypes(typ: Type) returns (x: Any)
-    ensures HasType(x, typ)
+  // predicate
 
-  function {:axiom} InterpLiteral(x: Literal): Any
-    ensures HasType(InterpLiteral(x), x.typ)
-  
-  predicate IsInt(x: Any) {
-    HasType(x, Int)
-  }
-
-  predicate IsBool(x: Any) {
-    HasType(x, Bool)
-  }
-
-  ghost predicate IsBoolSet(xs: iset<Any>) {
-    forall x <- xs :: IsBool(x)
-  }
-
-  ghost predicate IsIntSet(xs: iset<Any>) {
-    forall x <- xs :: IsInt(x)
-  }
-
-  function {:axiom} InterpInt(x: int): Any
-    ensures HasType(InterpInt(x), Int)
-
-  function {:axiom} InterpBool(x: bool): Any
-    ensures HasType(InterpBool(x), Bool)
-
-  function {:axiom} ToInt(x: Any): int
-    requires IsInt(x)
-    ensures InterpInt(ToInt(x)) == x
-
-  function {:axiom} ToBool(x: Any): bool
-    requires IsBool(x)
-    ensures InterpBool(ToBool(x)) == x
-
-  const True: Any := InterpBool(true)
-  const False: Any := InterpBool(false)
-
-  lemma {:axiom} TrueNotFalse()
-    ensures True != False
-
-  function Eql(x: Any, y: Any): Any
-  {
-    InterpBool(x == y)
-  }
-
-  function Neql(x: Any, y: Any): Any
-  {
-    InterpBool(x != y)
-  }
-
-  function Not(x: Any): Any
-    requires IsBool(x) 
-  {
-    InterpBool(!ToBool(x))
-  }
-
-  function LogicAnd(x: Any, y: Any): Any
-    requires IsBool(x)
-    requires IsBool(y)
-  {
-    InterpBool(ToBool(x) && ToBool(y))
-  }
-
-  function Implies(x: Any, y: Any): Any
-    requires IsBool(x) 
-    requires IsBool(y)
-  {
-    InterpBool(ToBool(x) ==> ToBool(y))
-  }
-
-  function Equiv(x: Any, y: Any): Any
-    requires IsBool(x) 
-    requires IsBool(y)
-  {
-    InterpBool(ToBool(x) <==> ToBool(y))
-  }
-
-  function Or(x: Any, y: Any): Any
-    requires IsBool(x) 
-    requires IsBool(y)
-  {
-    InterpBool(ToBool(x) || ToBool(y))
-  }
-
-  function Negate(x: Any): Any
-    requires IsInt(x) 
-  {
-    InterpInt(-ToInt(x))
-  }
-
-  function Plus(x: Any, y: Any): Any
-    requires IsInt(x) 
-    requires IsInt(y)
-  {
-    InterpInt(ToInt(x) + ToInt(y))
-  }
-
-  function Minus(x: Any, y: Any): Any
-    requires IsInt(x) 
-    requires IsInt(y) 
-  {
-    InterpInt(ToInt(x) - ToInt(y))
-  }
-
-  function Times(x: Any, y: Any): Any
-    requires IsInt(x) && IsInt(y) 
-  {
-    InterpInt(ToInt(x) * ToInt(y))
-  }
-
-  function Div(x: Any, y: Any): Any
-    requires IsInt(x) 
-    requires IsInt(y) 
-    requires ToInt(y) != 0
-  {
-    InterpInt(ToInt(x) / ToInt(y))
-  }
-
-  function Mod(x: Any, y: Any): Any
-    requires IsInt(x) 
-    requires IsInt(y) 
-    requires ToInt(y) != 0
-  {
-    InterpInt(ToInt(x) % ToInt(y))
-  }
-
-  function Less(x: Any, y: Any): Any
-    requires IsInt(x) 
-    requires IsInt(y)
-  {
-    InterpBool(ToInt(x) < ToInt(y))
-  }
-
-  function AtMost(x: Any, y: Any): Any
-    requires IsInt(x) 
-    requires IsInt(y)
-  {
-    InterpBool(ToInt(x) <= ToInt(y))
-  }
-
-  predicate HaveTypes(args: seq<Any>, sig: FunctionSig) {
-    |args| == |sig| && forall i :: 0 <= i < |args| ==> HasType(args[i], sig[i])
-  }
-
-  function {:axiom} InterpFunctionOn(func: Function, args: seq<Any>): Any
-    requires HaveTypes(args, func.sig)
-    ensures HasType(InterpFunctionOn(func, args), func.resultType)
-
-  lemma BoolIsTrueOrFalse(x: Any)
-    requires IsBool(x)
-    ensures x == True || x == False
-  {
-    assert x == InterpBool(ToBool(x));
-  }
 }
