src/Sound/Semantics/Omni.dfy
@@ -138,161 +138,161 @@ module Omni {
 
    */ 
 
-  ghost predicate SemSingle(s: Stmt, st: State, post: iset<State>) 
+  ghost predicate SemSingle(s: Stmt, st: State, post: iset<State>, m: M.Model) 
     requires s.Single()
     // reads *
   {
     match s
     case Check(e)       => 
       && e.IsDefinedOn(|st|) 
-      && (e.HoldsOn(st) &&  st in post)
+      && (e.HoldsOn(st, m) &&  st in post)
     case Assume(e)      => 
       && e.IsDefinedOn(|st|) 
-      && (e.HoldsOn(st) ==> st in post)
+      && (e.HoldsOn(st, m) ==> st in post)
     case Assign(x, v)   =>
         && x < |st|
         && v.IsDefinedOn(|st|)
-        && (v.Eval(st).Some? ==> st[x := v.Eval(st).value] in post)
+        && (v.Eval(st, m).Some? ==> st[x := v.Eval(st, m).value] in post)
     case Call(proc, args) =>
       && args.IsDefinedOn(|st|)
       && var callSt := args.Eval(st);
-        && (forall e <- proc.Pre :: e.IsDefinedOn(|callSt|) && e.HoldsOn(callSt))
+        && (forall e <- proc.Pre :: e.IsDefinedOn(|callSt|) && e.HoldsOn(callSt, m))
         && forall st': State :: (
           && st' in st.EqExcept(args.OutArgs())
           && var callSt' := args.Eval(st') + args.EvalOld(st);
-            (forall e <- proc.Post :: e.IsDefinedOn(|callSt'|) && e.HoldsOn(callSt')))
+            (forall e <- proc.Post :: e.IsDefinedOn(|callSt'|) && e.HoldsOn(callSt', m)))
               ==> st' in post
   }
 
-  ghost predicate PreservesInv(inv: iset<State>, body: Stmt, posts: Continuation)
+  ghost predicate PreservesInv(inv: iset<State>, body: Stmt, posts: Continuation, m: M.Model)
     // reads *
   { 
     forall st': State :: 
-      st' in inv ==> Sem(body, st', posts.UpdateHead(inv))
+      st' in inv ==> Sem(body, st', posts.UpdateHead(inv), m)
   }
 
-  ghost predicate Sem(s: Stmt, st: State, posts: Continuation) 
+  ghost predicate Sem(s: Stmt, st: State, posts: Continuation, m: M.Model) 
     // reads *
   {
-    if s.Single() then SemSingle(s, st, posts.head) else
+    if s.Single() then SemSingle(s, st, posts.head, m) else
     match s
-    case Seq(ss)        => SeqSem(ss, st, posts)
-    case Choice(s0, s1) => Sem(s0, st, posts) && Sem(s1, st, posts)
+    case Seq(ss)        => SeqSem(ss, st, posts, m)
+    case Choice(s0, s1) => Sem(s0, st, posts, m) && Sem(s1, st, posts, m)
     case NewScope(n, s) => 
-      forall vs: State :: |vs| == n ==> Sem(s, st.Update(vs), posts.UpdateAndAdd(n))
+      forall vs: State :: |vs| == n ==> Sem(s, st.Update(vs), posts.UpdateAndAdd(n), m)
     case Escape(l)      => |posts| > l && st in posts[l]
     case Loop(_, body) => 
       exists inv: iset<State> :: 
         && st in inv
         && forall st': State :: 
-          st' in inv ==> Sem(body, st', posts.UpdateHead(inv))
+          st' in inv ==> Sem(body, st', posts.UpdateHead(inv), m)
   }
 
-  greatest predicate RefSem(s: Stmt, st: State, posts: Continuation) 
+  greatest predicate RefSem(s: Stmt, st: State, posts: Continuation, m: M.Model) 
     reads *
   {
     match s
     case Check(e)       => 
-      e.RefHoldsOn(st) &&  st in posts.head
+      e.RefHoldsOn(st, m) &&  st in posts.head
     case Assume(e)      =>  
-      e.RefHoldsOn(st) ==> st in posts.head
+      e.RefHoldsOn(st, m) ==> st in posts.head
     case Assign(x, v)   => 
       && x < st.Size()
-      && (v.RefEval(st, iset v | true) ==>
-        v.RefEval(st, iset v {:trigger} | st.UpdateAt(x, v) in posts.head))
+      && (v.RefEval(st, (iset v | true), m) ==>
+        v.RefEval(st, (iset v {:trigger} | st.UpdateAt(x, v) in posts.head), m))
     case Call(proc, args) => 
-      && RefProcedureIsSound(proc)
+      && RefProcedureIsSound(proc, m)
       && args.IsDefinedOn(|st|)
       && var callSt := args.Eval(st);
-        && (forall e <- proc.Pre :: e.RefHoldsOn(callSt))
+        && (forall e <- proc.Pre :: e.RefHoldsOn(callSt, m))
         && forall st': State :: (
           && st' in st.EqExcept(args.OutArgs())
           && var callSt' := args.Eval(st') + args.EvalOld(st);
-            (forall e <- proc.Post :: e.RefHoldsOn(callSt')))
+            (forall e <- proc.Post :: e.RefHoldsOn(callSt', m)))
               ==> st' in posts.head
-    case Seq(ss)        => SeqRefSem(ss, st, posts)
-    case Choice(s0, s1) => RefSem(s0, st, posts) && RefSem(s1, st, posts)
+    case Seq(ss)        => SeqRefSem(ss, st, posts, m)
+    case Choice(s0, s1) => RefSem(s0, st, posts, m) && RefSem(s1, st, posts, m)
     case NewScope(n, s) => 
-      forall vs: State :: |vs| == n ==> RefSem(s, st.Update(vs), posts.UpdateAndAdd(n))
+      forall vs: State :: |vs| == n ==> RefSem(s, st.Update(vs), posts.UpdateAndAdd(n), m)
     case Escape(l)      => |posts| > l && st in posts[l]
-    case Loop(inv, body) => RefSem(Seq([body, Loop(inv, body)]), st, posts)
+    case Loop(inv, body) => RefSem(Seq([body, Loop(inv, body)]), st, posts, m)
   }
 
-  greatest predicate SeqRefSem(ss: seq<Stmt>, st: State, posts: Continuation) 
+  greatest predicate SeqRefSem(ss: seq<Stmt>, st: State, posts: Continuation, m: M.Model) 
     reads *
   {
     if ss == [] then st in posts.head else
     forall post': iset<State> :: 
-      (forall st: State :: SeqRefSem(ss[1..], st, posts) ==> st in post') ==> RefSem(ss[0], st, posts.UpdateHead(post'))
+      (forall st: State :: SeqRefSem(ss[1..], st, posts, m) ==> st in post') ==> RefSem(ss[0], st, posts.UpdateHead(post'), m)
   }
 
-  greatest predicate RefProcedureIsSound(proc: Procedure) 
+  greatest predicate RefProcedureIsSound(proc: Procedure, m: M.Model) 
     reads *
   {
     proc.Body.Some? ==>
-      forall st: State :: st in proc.PreSet() ==>
-        RefSem(proc.Body.value, st, SingleCont(proc.PostSet()))
+      forall st: State :: st in proc.PreSet(m) ==>
+        RefSem(proc.Body.value, st, SingleCont(proc.PostSet(m)), m)
   }
 
-  ghost predicate ProcedureIsSound(proc: Procedure) 
+  ghost predicate ProcedureIsSound(proc: Procedure, m: M.Model) 
     reads *
   {
     proc.Body.Some? ==>
-      forall st: State :: st in proc.PreSet() ==>
-        Sem(proc.Body.value, st, [proc.PostSet()])
+      forall st: State :: st in proc.PreSet(m) ==>
+        Sem(proc.Body.value, st, [proc.PostSet(m)], m)
   }
  
-  ghost function WP(s: Stmt, posts: Continuation) : iset<State> 
+  ghost function WP(s: Stmt, posts: Continuation, m: M.Model) : iset<State> 
     reads *
   {
-    iset st: State | Sem(s, st, posts)
+    iset st: State | Sem(s, st, posts, m)
   }
 
-  ghost predicate SeqSem(ss: seq<Stmt>, st: State, posts: Continuation) 
+  ghost predicate SeqSem(ss: seq<Stmt>, st: State, posts: Continuation, m: M.Model) 
     // reads *
   {
     if ss == [] then st in posts.head else
     forall post': iset<State> :: 
-      (forall st: State :: SeqSem(ss[1..], st, posts) ==> st in post') ==> Sem(ss[0], st, posts.UpdateHead(post'))
+      (forall st: State :: SeqSem(ss[1..], st, posts, m) ==> st in post') ==> Sem(ss[0], st, posts.UpdateHead(post'), m)
   }
 
-  ghost function SeqWP(ss: seq<Stmt>, cont: Continuation): iset<State> 
+  ghost function SeqWP(ss: seq<Stmt>, cont: Continuation, m: M.Model): iset<State> 
     // reads *
   {
-    iset st: State | SeqSem(ss, st, cont)
+    iset st: State | SeqSem(ss, st, cont, m)
   }
 
-  lemma SemCons(s: Stmt, st: State, posts: Continuation, posts': Continuation)
-    requires Sem(s, st, posts)
+  lemma SemCons(s: Stmt, st: State, posts: Continuation, posts': Continuation, m: M.Model)
+    requires Sem(s, st, posts, m)
     requires posts.Leq(posts')
-    ensures Sem(s, st, posts')
+    ensures Sem(s, st, posts', m)
   {
     match s
-    case Seq(ss) => SeqSemCons(ss, st, posts, posts');
+    case Seq(ss) => SeqSemCons(ss, st, posts, posts', m);
     case NewScope(n, s) => posts.LeqUpdateAndAdd(n, posts');
     case Loop(_, body) => forall inv { posts.LeqUpdateHead(inv, posts'); }
     case _ =>
   }
 
-  lemma SeqSemCons(ss: seq<Stmt>, st: State, posts: Continuation, posts': Continuation)
-    requires SeqSem(ss, st, posts)
+  lemma SeqSemCons(ss: seq<Stmt>, st: State, posts: Continuation, posts': Continuation, m: M.Model)
+    requires SeqSem(ss, st, posts, m)
     requires posts.Leq(posts')
-    ensures SeqSem(ss, st, posts')
+    ensures SeqSem(ss, st, posts', m)
   {
     if ss != [] {
       assert ss == [ss[0]] + ss[1..];
-      forall post': iset<State> | (forall st: State :: SeqSem(ss[1..], st, posts') ==> st in post') {
-        SemCons(ss[0], st, posts.UpdateHead(post'), posts'.UpdateHead(post'));
+      forall post': iset<State> | (forall st: State :: SeqSem(ss[1..], st, posts', m) ==> st in post') {
+        SemCons(ss[0], st, posts.UpdateHead(post'), posts'.UpdateHead(post'), m);
       }
     }
   }
 
-  lemma SemNest(s: Stmt, ss: seq<Stmt>, st: State, posts: Continuation) 
-    requires Sem(s, st, posts.UpdateHead(SeqWP(ss, posts)))
-    ensures SeqSem([s] + ss, st, posts)
+  lemma SemNest(s: Stmt, ss: seq<Stmt>, st: State, posts: Continuation, m: M.Model) 
+    requires Sem(s, st, posts.UpdateHead(SeqWP(ss, posts, m)), m)
+    ensures SeqSem([s] + ss, st, posts, m)
   {
-    forall post': iset<State> | (forall st: State :: SeqSem(ss, st, posts) ==> st in post') {
-      SemCons(s, st, posts.UpdateHead(SeqWP(ss, posts)), posts.UpdateHead(post'));
+    forall post': iset<State> | (forall st: State :: SeqSem(ss, st, posts, m) ==> st in post') {
+      SemCons(s, st, posts.UpdateHead(SeqWP(ss, posts, m)), posts.UpdateHead(post'), m);
     }
   }
 
@@ -304,106 +304,106 @@ module Omni {
   //   // assert ([s] + ss)[1..] == ss; 
   // }
 
-  lemma SeqSemSingle(s: Stmt, st: State, posts: Continuation)
-    requires SeqSem([s], st, posts)
-    ensures Sem(s, st, posts)
+  lemma SeqSemSingle(s: Stmt, st: State, posts: Continuation, m: M.Model)
+    requires SeqSem([s], st, posts, m)
+    ensures Sem(s, st, posts, m)
   {
     assert [s][0] == s;
     assert [s][1..] == [];
     assert posts == posts.UpdateHead(posts.head);
   }
 
-  lemma SeqSemNest(ss1: seq<Stmt>, ss2: seq<Stmt>, st: State, posts: Continuation) 
-    requires SeqSem(ss1 + ss2, st, posts)
-    ensures SeqSem(ss1, st, posts.UpdateHead(SeqWP(ss2, posts)))
+  lemma SeqSemNest(ss1: seq<Stmt>, ss2: seq<Stmt>, st: State, posts: Continuation, m: M.Model) 
+    requires SeqSem(ss1 + ss2, st, posts, m)
+    ensures SeqSem(ss1, st, posts.UpdateHead(SeqWP(ss2, posts, m)), m)
   {
     if ss1 == [] {
       assert [] + ss2 == ss2;
     } else {
       assert ([ss1[0]] + (ss1[1..] + ss2))[0] == ss1[0];
       assert ss1 + ss2 == [ss1[0]] + (ss1[1..] + ss2); 
-      assert forall post': iset<State> :: posts.UpdateHead(SeqWP(ss2, posts)).UpdateHead(post') == posts.UpdateHead(post');
+      assert forall post': iset<State> :: posts.UpdateHead(SeqWP(ss2, posts, m)).UpdateHead(post') == posts.UpdateHead(post');
     }
   }
 
-  lemma SeqLemma(ss1: seq<Stmt>, ss2: seq<Stmt>, st: State, posts: Continuation)
-    requires Sem(Seq(ss1 + ss2), st, posts)
-    ensures SeqSem([Seq(ss1)] + ss2, st, posts)
+  lemma SeqLemma(ss1: seq<Stmt>, ss2: seq<Stmt>, st: State, posts: Continuation, m: M.Model)
+    requires Sem(Seq(ss1 + ss2), st, posts, m)
+    ensures SeqSem([Seq(ss1)] + ss2, st, posts, m)
   {
-    SeqSemNest(ss1, ss2, st, posts);
-    SemNest(Seq(ss1), ss2, st, posts);
+    SeqSemNest(ss1, ss2, st, posts, m);
+    SemNest(Seq(ss1), ss2, st, posts, m);
   }
 
   function StateSize(st: State): nat {
     |st|
   }
 
-  lemma SemSeqLemma(ss: seq<Stmt>, st: State, posts: Continuation)
-    requires SeqSem(ss, st, posts)
-    ensures Sem(Seq(ss), st, posts)
+  lemma SemSeqLemma(ss: seq<Stmt>, st: State, posts: Continuation, m: M.Model)
+    requires SeqSem(ss, st, posts, m)
+    ensures Sem(Seq(ss), st, posts, m)
   {
 
   }
 
-  lemma SeqSemSingle'(s: Stmt, st: State, posts: Continuation)
-    requires Sem(s, st, posts)
-    ensures SeqSem([s], st, posts)
+  lemma SeqSemSingle'(s: Stmt, st: State, posts: Continuation, m: M.Model)
+    requires Sem(s, st, posts, m)
+    ensures SeqSem([s], st, posts, m)
   {
     assert [s][0] == s;
     assert [s][1..] == [];
     assert posts.UpdateHead(posts.head) == posts;
-    forall post': iset<State> | (forall st: State :: SeqSem([], st, posts) ==> st in post') 
-      ensures Sem(s, st, posts.UpdateHead(post')) {
-      SemCons(s, st, posts, posts.UpdateHead(post'));
+    forall post': iset<State> | (forall st: State :: SeqSem([], st, posts, m) ==> st in post') 
+      ensures Sem(s, st, posts.UpdateHead(post'), m) {
+      SemCons(s, st, posts, posts.UpdateHead(post'), m);
     }
   }
 
-  lemma SemLoopLemma(inv: Expr, body: Stmt, st: State, posts: Continuation, inv': iset<State>)
+  lemma SemLoopLemma(inv: Expr, body: Stmt, st: State, posts: Continuation, inv': iset<State>, m: M.Model)
     requires st in inv'
     requires forall st': State :: 
-      st' in inv' ==> Sem(body, st', posts.UpdateHead(inv'))
-    ensures Sem(Loop(inv, body), st, posts)
+      st' in inv' ==> Sem(body, st', posts.UpdateHead(inv'), m)
+    ensures Sem(Loop(inv, body), st, posts, m)
   {  }
 
-  lemma PreservesInvLemma(inv: iset<State>, body: Stmt, posts: Continuation)
-    requires PreservesInv(inv, body, posts)
+  lemma PreservesInvLemma(inv: iset<State>, body: Stmt, posts: Continuation, m: M.Model)
+    requires PreservesInv(inv, body, posts, m)
     ensures forall st': State :: 
-      st' in inv ==> Sem(body, st', posts.UpdateHead(inv))
+      st' in inv ==> Sem(body, st', posts.UpdateHead(inv), m)
   {  } 
 
-  lemma SemLoopUnroll(s: Stmt, inv: Expr, body: Stmt, st: State, posts: Continuation)
-    requires Sem(Loop(inv, body), st, posts)
-    ensures Sem(Seq([body, Loop(inv, body)]), st, posts)
+  lemma SemLoopUnroll(s: Stmt, inv: Expr, body: Stmt, st: State, posts: Continuation, m: M.Model)
+    requires Sem(Loop(inv, body), st, posts, m)
+    ensures Sem(Seq([body, Loop(inv, body)]), st, posts, m)
   {
-    var invEx :| st in invEx && PreservesInv(invEx, body, posts);
-    PreservesInvLemma(invEx, body, posts);
-    SemNest(body, [Loop(inv, body)], st, posts) by {
-      SemCons(body, st, posts.UpdateHead(invEx), posts.UpdateHead(SeqWP([Loop(inv, body)], posts))) by {
-        forall st: State | st in invEx ensures SeqSem([Loop(inv, body)], st, posts) {
-          SeqSemSingle'(Loop(inv, body), st, posts) by {
-            SemLoopLemma(inv, body, st, posts, invEx);
+    var invEx :| st in invEx && PreservesInv(invEx, body, posts, m);
+    PreservesInvLemma(invEx, body, posts, m);
+    SemNest(body, [Loop(inv, body)], st, posts, m) by {
+      SemCons(body, st, posts.UpdateHead(invEx), posts.UpdateHead(SeqWP([Loop(inv, body)], posts, m)), m) by {
+        forall st: State | st in invEx ensures SeqSem([Loop(inv, body)], st, posts, m) {
+          SeqSemSingle'(Loop(inv, body), st, posts, m) by {
+            SemLoopLemma(inv, body, st, posts, invEx, m);
           }
         }
       }
     }
   }
 
-  greatest lemma SemSound(s: Stmt, st: State, posts: Continuation, procs: set<Procedure>, funs: set<Function>)
-    requires Sem(s, st, posts)
+  greatest lemma SemSound(s: Stmt, st: State, posts: Continuation, procs: set<Procedure>, funs: set<Function>, m: M.Model)
+    requires Sem(s, st, posts, m)
     requires s.ProceduresCalled() <= procs
     requires s.FunctionsCalled() <= funs
     requires forall p <- procs :: p.ProceduresCalled() <= procs
     requires forall p <- procs :: p.FunctionsCalled() <= funs
     requires forall f <- funs :: f.FunctionsCalled() <= funs
-    requires forall p <- procs :: ProcedureIsSound(p)
-    requires forall f <- funs :: f.IsSound()
-    ensures RefSem(s, st, posts)
+    requires forall p <- procs :: ProcedureIsSound(p, m)
+    requires forall f <- funs :: f.IsSound(m)
+    ensures RefSem(s, st, posts, m)
   {
       match s
-      case Seq(ss) => SeqSemSound(ss, st, posts, procs, funs);
+      case Seq(ss) => SeqSemSound(ss, st, posts, procs, funs, m);
       case Loop(inv, body) => 
-        SemLoopUnroll(s, inv, body, st, posts);
-        SemSound(Seq([body, Loop(inv, body)]), st, posts, procs, funs) by {
+        SemLoopUnroll(s, inv, body, st, posts, m);
+        SemSound(Seq([body, Loop(inv, body)]), st, posts, procs, funs, m) by {
           forall p <- SeqProceduresCalled([body, Loop(inv, body)])
             ensures p in s.ProceduresCalled()
           {
@@ -430,185 +430,185 @@ module Omni {
         }
       case Call(proc, args) => 
         var callSt := args.Eval(st);
-        forall e <- proc.Pre ensures e.RefHoldsOn(callSt) {
-          e.HoldsOnSound(callSt, funs) by {
+        forall e <- proc.Pre ensures e.RefHoldsOn(callSt, m) {
+          e.HoldsOnSound(callSt, funs, m) by {
             SeqExprFunctionsCalledIn(proc.Pre, e);
           }
         }
         forall post <- proc.Post, st 
-          ensures post.RefHoldsOn(st) == (post.IsDefinedOn(st.Size()) && post.HoldsOn(st))
+          ensures post.RefHoldsOn(st, m) == (post.IsDefinedOn(st.Size()) && post.HoldsOn(st, m))
         {
-          post.HoldsOnSound(st, funs) by {
+          post.HoldsOnSound(st, funs, m) by {
             SeqExprFunctionsCalledIn(proc.Post, post);
           }
         }
-        assert ProcedureIsSound(proc);
-        ProcedureIsSoundSound(proc, procs, funs);
-      case Assume(e) => e.HoldsOnSound(st, funs);
-      case Check(e) => e.HoldsOnSound(st, funs);
+        assert ProcedureIsSound(proc, m);
+        ProcedureIsSoundSound(proc, procs, funs, m);
+      case Assume(e) => e.HoldsOnSound(st, funs, m);
+      case Check(e) => e.HoldsOnSound(st, funs, m);
       case Assign(x, v) =>
-        assert (v.RefEval(st, iset v {:trigger} | true) ==>
-        v.RefEval(st, iset v {:trigger} | st.UpdateAt(x, v) in posts.head)) by {
-          if v.RefEval(st, iset v {:trigger} | true) {
-            v.EvalComplete(st, iset v {:trigger} | true);
-            v.EvalSound(st, funs, iset v {:trigger} | st.UpdateAt(x, v) in posts.head);
+        assert (v.RefEval(st, (iset v {:trigger} | true), m) ==>
+        v.RefEval(st, (iset v {:trigger} | st.UpdateAt(x, v) in posts.head), m)) by {
+          if v.RefEval(st, (iset v {:trigger} | true), m) {
+            v.EvalComplete(st, (iset v {:trigger} | true), m);
+            v.EvalSound(st, funs, (iset v {:trigger} | st.UpdateAt(x, v) in posts.head), m);
           }
         }
       case _ =>
   }
 
-  greatest lemma ProcedureIsSoundSound(proc: Procedure, procs: set<Procedure>, funs: set<Function>)
-    requires ProcedureIsSound(proc)
+  greatest lemma ProcedureIsSoundSound(proc: Procedure, procs: set<Procedure>, funs: set<Function>, m: M.Model)
+    requires ProcedureIsSound(proc, m)
     requires proc.ProceduresCalled() <= procs
     requires proc.FunctionsCalled() <= funs
-    requires forall f <- funs :: f.IsSound()
+    requires forall f <- funs :: f.IsSound(m)
     requires forall f <- funs :: f.FunctionsCalled() <= funs
     requires forall p <- procs :: p.ProceduresCalled() <= procs
-    requires forall p <- procs :: ProcedureIsSound(p)
+    requires forall p <- procs :: ProcedureIsSound(p, m)
     requires forall p <- procs :: p.FunctionsCalled() <= funs
-    ensures RefProcedureIsSound(proc)
+    ensures RefProcedureIsSound(proc, m)
   {
     if proc.Body.Some? {
-      forall st: State | st in proc.PreSet()
-        ensures RefSem(proc.Body.value, st, SingleCont(proc.PostSet())) {
-        SemSound(proc.Body.value, st, SingleCont(proc.PostSet()), procs, funs);
+      forall st: State | st in proc.PreSet(m)
+        ensures RefSem(proc.Body.value, st, SingleCont(proc.PostSet(m)), m) {
+        SemSound(proc.Body.value, st, SingleCont(proc.PostSet(m)), procs, funs, m);
       }
     }
   }
 
-  greatest lemma SeqSemSound(ss: seq<Stmt>, st: State, posts: Continuation, procs: set<Procedure>, funs: set<Function>)
-    requires SeqSem(ss, st, posts)
+  greatest lemma SeqSemSound(ss: seq<Stmt>, st: State, posts: Continuation, procs: set<Procedure>, funs: set<Function>, m: M.Model)
+    requires SeqSem(ss, st, posts, m)
     requires SeqProceduresCalled(ss) <= procs
     requires SeqFunctionsCalled(ss) <= funs
     requires forall p <- procs :: p.ProceduresCalled() <= procs
     requires forall f <- funs :: f.FunctionsCalled() <= funs
-    requires forall p <- procs :: ProcedureIsSound(p)
+    requires forall p <- procs :: ProcedureIsSound(p, m)
     requires forall p <- procs :: p.FunctionsCalled() <= funs
-    requires forall f <- funs :: f.IsSound()
-    ensures SeqRefSem(ss, st, posts)
+    requires forall f <- funs :: f.IsSound(m)
+    ensures SeqRefSem(ss, st, posts, m)
   {
     if ss != [] {
-      forall post': iset<State> | (forall st: State :: SeqRefSem(ss[1..], st, posts) ==> st in post') 
-        ensures RefSem(ss[0], st, posts.UpdateHead(post')) {
-        SemSound(ss[0], st, posts.UpdateHead(post'), procs, funs);
+      forall post': iset<State> | (forall st: State :: SeqRefSem(ss[1..], st, posts, m) ==> st in post') 
+        ensures RefSem(ss[0], st, posts.UpdateHead(post'), m) {
+        SemSound(ss[0], st, posts.UpdateHead(post'), procs, funs, m);
       }
     }
   }
 
-  lemma SemSoundProc(proc: Procedure, procs: set<Procedure>, funs: set<Function>)
+  lemma SemSoundProc(proc: Procedure, procs: set<Procedure>, funs: set<Function>, m: M.Model)
     requires proc in procs
     requires proc.ProceduresCalled() <= procs
     requires proc.FunctionsCalled() <= funs
-    requires forall f <- funs :: f.IsSound()
+    requires forall f <- funs :: f.IsSound(m)
     requires forall f <- funs :: f.FunctionsCalled() <= funs
     requires forall p <- procs :: p.ProceduresCalled() <= procs
     requires forall p <- procs :: p.FunctionsCalled() <= funs
-    requires forall p <- procs :: ProcedureIsSound(p)
-    ensures RefProcedureIsSound(proc)
+    requires forall p <- procs :: ProcedureIsSound(p, m)
+    ensures RefProcedureIsSound(proc, m)
   {
     if proc.Body.Some? {
-      forall st: State | st in proc.PreSet()
-        ensures RefSem(proc.Body.value, st, SingleCont(proc.PostSet())) {
-        SemSound(proc.Body.value, st, SingleCont(proc.PostSet()), procs, funs);
+      forall st: State | st in proc.PreSet(m)
+        ensures RefSem(proc.Body.value, st, SingleCont(proc.PostSet(m)), m) {
+        SemSound(proc.Body.value, st, SingleCont(proc.PostSet(m)), procs, funs, m);
       }
     }
   }
 
-  lemma SemSoundProcs(procs: set<Procedure>, funcs: set<Function>)
+  lemma SemSoundProcs(procs: set<Procedure>, funcs: set<Function>, m: M.Model)
     requires forall proc <- procs :: proc.Valid()
-    requires forall proc <- procs :: ProcedureIsSound(proc)
-    requires forall func <- funcs :: func.IsSound()
+    requires forall proc <- procs :: ProcedureIsSound(proc, m)
+    requires forall func <- funcs :: func.IsSound(m)
     requires forall proc <- procs :: proc.ProceduresCalled() <= procs
     requires forall proc <- procs :: proc.FunctionsCalled() <= funcs
     requires forall func <- funcs :: func.FunctionsCalled() <= funcs
-    ensures  forall proc <- procs :: RefProcedureIsSound(proc)
+    ensures  forall proc <- procs :: RefProcedureIsSound(proc, m)
   {
     forall proc <- procs 
-      ensures RefProcedureIsSound(proc) {
-      SemSoundProc(proc, procs, funcs);
+      ensures RefProcedureIsSound(proc, m) {
+      SemSoundProc(proc, procs, funcs, m);
     }
   }
 
-  lemma SemLoopWithCont(inv: Expr, body: Stmt, cont: seq<Stmt>, st: State, posts: Continuation, inv': iset<State>)
+  lemma SemLoopWithCont(inv: Expr, body: Stmt, cont: seq<Stmt>, st: State, posts: Continuation, inv': iset<State>, m: M.Model)
     requires st in inv'
     requires forall st': State :: 
-      st' in inv' ==> Sem(body, st', posts.UpdateHead(inv'))
-    ensures SeqSem([Loop(inv, body)] + cont, st, posts)
+      st' in inv' ==> Sem(body, st', posts.UpdateHead(inv'), m)
+    ensures SeqSem([Loop(inv, body)] + cont, st, posts, m)
   {
-    SemNest(Loop(inv, body), cont, st, posts) by {
-      SemLoopLemma(inv, body, st, posts.UpdateHead(SeqWP(cont, posts)), inv') by {
-        assert posts.UpdateHead(SeqWP(cont, posts)).UpdateHead(inv') == posts.UpdateHead(inv');
+    SemNest(Loop(inv, body), cont, st, posts, m) by {
+      SemLoopLemma(inv, body, st, posts.UpdateHead(SeqWP(cont, posts, m)), inv', m) by {
+        assert posts.UpdateHead(SeqWP(cont, posts, m)).UpdateHead(inv') == posts.UpdateHead(inv');
       }
     }
   }
   
-  lemma SemConsDepthLemma(s: Stmt, st: State, posts: Continuation, posts': Continuation, n: nat)
-    requires Sem(s, st, posts)
+  lemma SemConsDepthLemma(s: Stmt, st: State, posts: Continuation, posts': Continuation, n: nat, m: M.Model)
+    requires Sem(s, st, posts, m)
     requires posts.LeqDepth(posts', n)
     requires s.JumpsDefinedOn(n)
-    ensures Sem(s, st, posts')
+    ensures Sem(s, st, posts', m)
   {
     match s
-    case Seq(ss) => SeqSemConsDepthLemma(ss, st, posts, posts', n);
-    case NewScope(m, s) => 
-      forall vs: State | |vs| == m 
-        ensures Sem(s, st.Update(vs), posts'.UpdateAndAdd(m)) {
+    case Seq(ss) => SeqSemConsDepthLemma(ss, st, posts, posts', n, m);
+    case NewScope(k, s) => 
+      forall vs: State | |vs| == k
+        ensures Sem(s, st.Update(vs), posts'.UpdateAndAdd(k), m) {
         if s.JumpDepth() == 0 {
-          SemConsDepthLemma(s, st.Update(vs), posts.UpdateAndAdd(m), posts'.UpdateAndAdd(m), 0);
+          SemConsDepthLemma(s, st.Update(vs), posts.UpdateAndAdd(k), posts'.UpdateAndAdd(k), 0, m);
         } else {
-          posts.LeqDepthUpdateAndAdd(m, posts', n);
-          SemConsDepthLemma(s, st.Update(vs), posts.UpdateAndAdd(m), posts'.UpdateAndAdd(m), n + 1);
+          posts.LeqDepthUpdateAndAdd(k, posts', n);
+          SemConsDepthLemma(s, st.Update(vs), posts.UpdateAndAdd(k), posts'.UpdateAndAdd(k), n + 1, m);
         }
       }
     case Loop(_, body) => forall inv { posts.LeqDepthUpdateHead(inv, posts', n); }
     case _ =>
   }
 
-  lemma SeqSemConsDepthLemma(ss: seq<Stmt>, st: State, posts: Continuation, posts': Continuation, n: nat)
-    requires SeqSem(ss, st, posts)
+  lemma SeqSemConsDepthLemma(ss: seq<Stmt>, st: State, posts: Continuation, posts': Continuation, n: nat, m: M.Model)
+    requires SeqSem(ss, st, posts, m)
     requires posts.LeqDepth(posts', n)
     requires SeqJumpsDefinedOn(ss, n)
-    ensures SeqSem(ss, st, posts')
+    ensures SeqSem(ss, st, posts', m)
   {
     if ss != [] {
       assert ss == [ss[0]] + ss[1..];
-      forall post': iset<State> | (forall st: State :: SeqSem(ss[1..], st, posts') ==> st in post') {
-        SemConsDepthLemma(ss[0], st, posts.UpdateHead(post'), posts'.UpdateHead(post'), n);
+      forall post': iset<State> | (forall st: State :: SeqSem(ss[1..], st, posts', m) ==> st in post') {
+        SemConsDepthLemma(ss[0], st, posts.UpdateHead(post'), posts'.UpdateHead(post'), n, m);
       }
     }
   }
 
-  lemma InvSem(inv: Expr, body: Stmt, st: State, posts: Continuation, stmt: Stmt)
-    requires SeqSem([Assume(inv), body, Check(inv), stmt], st, posts)
-    requires st in inv.Sem()
-    ensures Sem(body, st, posts.UpdateHead(inv.Sem()))
+  lemma InvSem(inv: Expr, body: Stmt, st: State, posts: Continuation, stmt: Stmt, m: M.Model)
+    requires SeqSem([Assume(inv), body, Check(inv), stmt], st, posts, m)
+    requires st in inv.Sem(m)
+    ensures Sem(body, st, posts.UpdateHead(inv.Sem(m)), m)
   {
-    SeqSemNest([Assume(inv)], [body, Check(inv), stmt], st, posts);
-    SeqSemSingle(Assume(inv), st, posts.UpdateHead(SeqWP([body, Check(inv), stmt], posts)));
-    assert SeqSem([body, Check(inv), stmt], st, posts);
-    SeqSemNest([body], [Check(inv), stmt], st, posts);
-    SeqSemSingle(body, st, posts.UpdateHead(SeqWP([Check(inv), stmt], posts)));
-    SemCons(body, st, posts.UpdateHead(SeqWP([Check(inv), stmt], posts)), posts.UpdateHead(inv.Sem())) by {
-      forall st': State | SeqSem([Check(inv), stmt], st', posts) ensures st' in inv.Sem() {
-        SeqSemNest([Check(inv)], [stmt], st', posts);
-        SeqSemSingle(Check(inv), st', posts.UpdateHead(SeqWP([stmt], posts)));
+    SeqSemNest([Assume(inv)], [body, Check(inv), stmt], st, posts, m);
+    SeqSemSingle(Assume(inv), st, posts.UpdateHead(SeqWP([body, Check(inv), stmt], posts, m)), m);
+    assert SeqSem([body, Check(inv), stmt], st, posts, m);
+    SeqSemNest([body], [Check(inv), stmt], st, posts, m);
+    SeqSemSingle(body, st, posts.UpdateHead(SeqWP([Check(inv), stmt], posts, m)), m);
+    SemCons(body, st, posts.UpdateHead(SeqWP([Check(inv), stmt], posts, m)), posts.UpdateHead(inv.Sem(m)), m) by {
+      forall st': State | SeqSem([Check(inv), stmt], st', posts, m) ensures st' in inv.Sem(m) {
+        SeqSemNest([Check(inv)], [stmt], st', posts, m);
+        SeqSemSingle(Check(inv), st', posts.UpdateHead(SeqWP([stmt], posts, m)), m);
       }
     }
   }
 
-  lemma SemPostCheck'Lemma(proc: Procedure, st: State, posts: Continuation, p: seq<Expr>)
+  lemma SemPostCheck'Lemma(proc: Procedure, st: State, posts: Continuation, p: seq<Expr>, m: M.Model)
     requires forall e <- p :: e.IsDefinedOn(|proc.Parameters| + proc.NumInOutArgs())
-    requires SeqSem(proc.PostCheck'(p), st, posts)
-    ensures forall e <- p :: e.IsDefinedOn(|st|) && e.HoldsOn(st)
+    requires SeqSem(proc.PostCheck'(p), st, posts, m)
+    ensures forall e <- p :: e.IsDefinedOn(|st|) && e.HoldsOn(st, m)
   {
     if p != [] {
       forall e <- p 
-        ensures e.IsDefinedOn(|st|) && e.HoldsOn(st) {
-        SeqSemNest([Check(p[0])], proc.PostCheck'(p[1..]), st, posts) by {
+        ensures e.IsDefinedOn(|st|) && e.HoldsOn(st, m) {
+        SeqSemNest([Check(p[0])], proc.PostCheck'(p[1..]), st, posts, m) by {
           assert forall e <- p[1..] :: e in p;
         }
         if e in p[1..] {
-          SemPostCheck'Lemma(proc, st, posts, p[1..]) by {
+          SemPostCheck'Lemma(proc, st, posts, p[1..], m) by {
             forall e <- p[1..]
               ensures e.IsDefinedOn(|proc.Parameters| + proc.NumInOutArgs()) {
               assert e in p;
@@ -619,11 +619,11 @@ module Omni {
     }
   }
 
-  lemma SemPostCheckLemma(proc: Procedure, st: State, posts: Continuation)
+  lemma SemPostCheckLemma(proc: Procedure, st: State, posts: Continuation, m: M.Model)
     requires proc.Valid()
-    requires SeqSem(proc.PostCheck(), st, posts)
-    ensures forall e <- proc.Post :: e.IsDefinedOn(|st|) && e.HoldsOn(st)
+    requires SeqSem(proc.PostCheck(), st, posts, m)
+    ensures forall e <- proc.Post :: e.IsDefinedOn(|st|) && e.HoldsOn(st, m)
   {
-    SemPostCheck'Lemma(proc, st, posts, proc.Post);
+    SemPostCheck'Lemma(proc, st, posts, proc.Post, m);
   }
 }
